bedrock2/src/Examples/MultipleReturnValues.v
@@ -14,14 +14,14 @@ Section MultipleReturnValues.
   Let x : varname := "x".
   Let y : varname := "y".
 
-  Example addsub := ((a::b::nil), (x::y::nil), bedrock_func(
+  Example addsub := ((a::b::nil), (x::y::nil), bedrock_func_body:(
     x = a + b;
     y = a - b
   )).
 
   Let ret : varname := "ret".
 
-  Example addsub_test := (@nil varname, ("ret"::nil)%list, bedrock_func(
+  Example addsub_test := (@nil varname, ("ret"::nil)%list, bedrock_func_body:(
     cmd.call (ret::ret::nil)%list "addsub" (expr.literal 14::expr.literal 7::nil)%list;
     ret = (ret - 7)
   )).
